theories/test.v
@@ -1,0 +1,14 @@
+From diris.heap_lang Require Export notation.
+From iris.proofmode Require Export tactics.
+From iris.heap_lang Require Import proofmode.
+
+
+Set Default Proof Using "Type".
+
+Definition new_lock : val := λ: <>, ref #false.
+Definition lock : val := λ: "x", WAS "x" #false #true.
+Definition unlock : val := λ: "x", "x" <- #true.
+
+Lemma lock_spec1 x a : {{{ x ↦ a }}} lock x {{{ RET #(); x ↦ #true }}}.
+Proof.
+Qed.
